\section{Exercise 4}
\[
	V = \{(w,x,y,z) \in \mathbb{R}^4 | w+2x = 0\}
\]

\begin{align*}
	u_1 & = (2,-1,1,2) &
	u_2 & = (-2,1,2,0) &
	u_3 & = (0,0,2,1)
\end{align*}

\subsection{Part a}
To check whether $u_1,u_2,u_3$ span $V$ we must find whether all vectors in $V$ can be written as a linear combination of $u_1,u_2,u_3$. So, with $w=-2x$:
\[
	(-2x,x,y,z) = a(2,-1,1,2) + b(-2,1,2,0) + c(0,0,2,1)
\]

Create a system of equations:
\begin{align*}
	2a-2b   & = -2x \\
	-a+b    & = x   \\
	a+2b+2c & = y   \\
	2a+c    & = z
\end{align*}

We can then solve for each of the variables. Use the second to $b$:
\begin{align*}
	b & = x+a \\
\end{align*}

We can check this by substituting into the first:
\begin{align*}
	2a-2(x+a) & = -2x \\
	2a-2x-2a  & = -2x \\
	-2x       & = -2x
\end{align*}

This is true, so we can continue to solve for $c$:
\begin{align*}
	2a+c & = z   \\
	2a   & = z-c \\
	z-2a & = c
\end{align*}

We can then substitute $b$ and $c$ into the third equation:
\begin{align*}
	a+2(x+a)+2(z-2a) & = y        \\
	a+2x+2a+2z-4a    & = y        \\
	-a+2x+2z         & = y
	\intertext{Solve for $a$}
	a                & = -y+2x+2z \\
\end{align*}

Status now is:
\begin{align*}
	a & = -y+2x+2z \\
	b & = x+a      \\
	c & = z-2a
\end{align*}

Substitute $a$ into $b$:
\begin{align*}
	b & = x+(-y+2x+2z) \\
	b & = x-y+2x+2z    \\
	b & = -y+3x+2z
\end{align*}

Substitute $a$ into $c$:
\begin{align*}
	c & = z-2(-y+2x+2z) \\
	c & = z+2y-4x-4z    \\
	c & = 2y-4x-3z
\end{align*}

So we have:
\begin{align*}
	a & = -y+2x+2z = 2x-y+2z   \\
	b & = -y+3x+2z = 3x-y+2z   \\
	c & = 2y-4x-3z = -4x+2y-3z
\end{align*}

So:
\[
	(-2x,x,y,z) = (2x-y+2z)u_1 + (3x-y+2z)u_2 + (-4x+2y-3z)u_3
\]


