\section{Exercise 6}
\question{
	Let $X,Y$ be random variables with joint PDF given by
	\[
		f_{X,Y}(x,y) =  \begin{cases}
			\frac{3}{7}(xy^2+3x^2) & \text{for } 0 \leq x \leq 1 \text{ and } -1 \leq y \leq 1 \\
			0                      & \text{else}
		\end{cases}
	\]
}

\section{Part a}
\question{
	Compute the conditional PDF $f_{Y|X}(x|y)$.
}

We can find the conditional PDF by using the formula:
\[
	f_{Y|X}(y|x) = \frac{f_{X,Y}(x,y)}{f_X(x)}
\]

We can find $f_X(x)$ by integrating $f_{X,Y}(x,y)$ over $y$:
\begin{align*}
	f_X(x) & = \int_{-\infty}^{\infty} f_{X,Y}(x,y)\ dy                                \\
	       & = \int_{-1}^{1} \frac{3}{7}(xy^2+3x^2)\ dy                                \\
	       & = \frac{3x}{7} \left(\int_{-1}^{1} y^2\ dy+3x^2\int_{-1}^{1} 1\ dy\right) \\
	       & = \frac{3x}{7} \left(\frac{y^3}{3}+3x^2y\right)                           \\
	       & = \frac{xy^3}{7}+\frac{9x^2y}{7}                                          \\
	       & = \frac{xy^3 + 9x^2y}{7}                                                  \\
	       & = \left[\frac{xy (y^2 + 9x)}{7}\right]^{-1}_1                             \\
	       & = \frac{x\cdot 1 (1^2 + 9x)}{7} - \frac{x\cdot -1 (-1^2 + 9x)}{7}         \\
	       & = \frac{9x^2}{7} - \left(-\frac{x (9x-1)}{7}\right)                       \\
	       & = \frac{9x^2}{7} + \frac{9x^2-x}{7}                                       \\
	       & = \frac{9x^2 + 9x^2-x}{7}                                                 \\
	       & = \frac{2(9x^2+x)}{7}                                                     \\
\end{align*}

We can then find the conditional PDF:
\begin{align*}
	f_{Y|X}(y|x) & = \frac{f_{X,Y}(x,y)}{f_X(x)}                        \\
	             & = \frac{\frac{3}{7}(xy^2+3x^2)}{\frac{2(9x^2+x)}{7}} \\
	             & = \frac{3(xy^2+3x^2)}{2(9x^2+x)}                     \\
	             & = \frac{3(xy^2+3x^2)}{2x(9x+1)}                      \\
	             & = \frac{3(x(y^2+3x))}{2x(9x+1)}                      \\
	             & = \frac{3(y^2+3x)}{2(9x+1)}                          \\
\end{align*}
