\section{Exercise 5}
For this problem, consider two continuous random variables $X$ and $Y$ with joint PDF given as

\[
	f(x,y) = \begin{cases}
		\frac{3}{2}(x^2y +x) & \text{if } 0 \leq x \leq 1 \text{ and } 0 \leq y \leq 1 \\
		0                    & \text{otherwise}
	\end{cases}
\]

\subsection{Part a}
\question{
	Compute the probability that $X \leq Y$
}

To compute the probability that $X \leq Y$ we need to compute the double integral of the joint PDF over the region where $X \leq Y$. This region is the triangle where $0 \leq x \leq 1$ and $x \leq y \leq 1$. We can then compute the integral as
\begin{align*}
	P(X\leq Y) & = \int_{0}^{1}\int_{x}^{1} \frac{3}{2}(x^2y + x)\, dy\, dx                                          \\
	           & = \int_{0}^{1} \frac{3x^2}{2} \int_{x}^{1}y\, dy + \frac{3x}{2} \int_{x}^{1}1\, dy\, dx             \\
	           & = \int_{0}^{1} \left[\frac{3x^2}{2} \frac{y^2}{2} + \frac{3x}{2} y\right]^1_x dx                    \\
	           & = \int_{0}^{1} \left[\frac{3x^2y^2}{4} + \frac{3xy}{2}\right]^1_x dx                                \\
	           & = \int_{0}^{1} \left[\frac{3x^2y^2}{4} + \frac{6xy}{4}\right]^1_x dx                                \\
	           & = \int_{0}^{1} \left[\frac{3x^2y^2+6xy}{4}\right]^1_x dx                                            \\
	           & = \int_{0}^{1} \frac{3x^2\cdot 1^2+6x\cdot 1}{4} -  \frac{3x^2\cdot x^2+6x\cdot x}{4}\,dx           \\
	           & = \int_{0}^{1} \frac{3x^2+6x}{4} -  \frac{3x^4+6x^2}{4}\,dx                                         \\
	           & = \int_{0}^{1} \frac{3x^2+6x-(3x^4+6x^2)}{4}\,dx                                                    \\
	           & = \int_{0}^{1} \frac{-3x^4+3x^2-6x^2+6x}{4}\,dx                                                     \\
	           & =  -\frac{3}{4}\int_{0}^{1}x^4\, dx-\frac{3}{4}\int_{0}^{1}x^2\, dx + \frac{6}{4}\int_{0}^{1}x\, dx \\
	           & =  \left[-\frac{3}{4}\frac{x^5}{5}-\frac{3}{4}\frac{x^3}{3} + \frac{6}{4}\frac{x^2}{2}\right]_0^1   \\
	           & =  \left[-\frac{3x^5}{20}-\frac{3x^3}{12} + \frac{6x^2}{8}\right]_0^1                               \\
	           & =  \left[-\frac{3x^5}{20}-\frac{x^3}{4} + \frac{3x^2}{4}\right]_0^1                                 \\
	           & =  \left[-\frac{3x^5}{20}-\frac{x^3+3x^2}{4}\right]_0^1                                             \\
	           & =  \left[-\frac{3x^5}{20}-\frac{5x^3+15x^2}{20}\right]_0^1                                          \\
	           & =  \left[-\frac{3x^5 - (5x^3+15x^2)}{20}\right]_0^1                                                 \\
	           & =  \left[-\frac{x^2(3x^3 + 5x-15)}{20}\right]_0^1                                                   \\
	           & =  -\frac{1^2(3\cdot1^3 + 5\cdot 1-15)}{20}-\frac{0^2(3\cdot 0^3 + 5\cdot 0-15)}{20}                \\
	           & =  -\frac{3 + 5-15}{20}                                                                             \\
	           & =  \frac{7}{20}                                                                                     \\
\end{align*}
